verity/artifacts/sphincs-kernel/MerkleKernel.yul
@@ -108,6 +108,70 @@ object "MerkleKernel" {
                         mstore(0, level3)
                         return(0, 32)
                     }
+                    case 0x64cf5e33 {
+                        /* previewPackedPath() */
+                        if callvalue() {
+                            revert(0, 0)
+                        }
+                        if lt(calldatasize(), 196) {
+                            revert(0, 0)
+                        }
+                        if lt(calldatasize(), 196) {
+                            revert(0, 0)
+                        }
+                        let leaf := calldataload(4)
+                        let sibling0 := calldataload(36)
+                        let sibling1 := calldataload(68)
+                        let sibling2 := calldataload(100)
+                        let sibling3 := calldataload(132)
+                        let directions := calldataload(164)
+                        let sibling0OnLeft := iszero(eq(and(directions, 1), 0))
+                        let sibling1OnLeft := iszero(eq(and(shr(1, directions), 1), 0))
+                        let sibling2OnLeft := iszero(eq(and(shr(2, directions), 1), 0))
+                        let sibling3OnLeft := iszero(eq(and(shr(3, directions), 1), 0))
+                        let level0 := 0
+                        {
+                            let __ite_cond := sibling0OnLeft
+                            if __ite_cond {
+                                level0 := add(mul(sibling0, 65537), add(mul(leaf, 257), 97))
+                            }
+                            if iszero(__ite_cond) {
+                                level0 := add(mul(leaf, 65537), add(mul(sibling0, 257), 97))
+                            }
+                        }
+                        let level1 := 0
+                        {
+                            let __ite_cond := sibling1OnLeft
+                            if __ite_cond {
+                                level1 := add(mul(sibling1, 65537), add(mul(level0, 257), 97))
+                            }
+                            if iszero(__ite_cond) {
+                                level1 := add(mul(level0, 65537), add(mul(sibling1, 257), 97))
+                            }
+                        }
+                        let level2 := 0
+                        {
+                            let __ite_cond := sibling2OnLeft
+                            if __ite_cond {
+                                level2 := add(mul(sibling2, 65537), add(mul(level1, 257), 97))
+                            }
+                            if iszero(__ite_cond) {
+                                level2 := add(mul(level1, 65537), add(mul(sibling2, 257), 97))
+                            }
+                        }
+                        let level3 := 0
+                        {
+                            let __ite_cond := sibling3OnLeft
+                            if __ite_cond {
+                                level3 := add(mul(sibling3, 65537), add(mul(level2, 257), 97))
+                            }
+                            if iszero(__ite_cond) {
+                                level3 := add(mul(level2, 65537), add(mul(sibling3, 257), 97))
+                            }
+                        }
+                        mstore(0, level3)
+                        return(0, 32)
+                    }
                     case 0x5bd839a5 {
                         /* verifyPath() */
                         if callvalue() {
@@ -129,6 +193,71 @@ object "MerkleKernel" {
                         let sibling2OnLeft := iszero(iszero(calldataload(228)))
                         let sibling3OnLeft := iszero(iszero(calldataload(260)))
                         let stored := sload(0)
+                        let level0 := 0
+                        {
+                            let __ite_cond := sibling0OnLeft
+                            if __ite_cond {
+                                level0 := add(mul(sibling0, 65537), add(mul(leaf, 257), 97))
+                            }
+                            if iszero(__ite_cond) {
+                                level0 := add(mul(leaf, 65537), add(mul(sibling0, 257), 97))
+                            }
+                        }
+                        let level1 := 0
+                        {
+                            let __ite_cond := sibling1OnLeft
+                            if __ite_cond {
+                                level1 := add(mul(sibling1, 65537), add(mul(level0, 257), 97))
+                            }
+                            if iszero(__ite_cond) {
+                                level1 := add(mul(level0, 65537), add(mul(sibling1, 257), 97))
+                            }
+                        }
+                        let level2 := 0
+                        {
+                            let __ite_cond := sibling2OnLeft
+                            if __ite_cond {
+                                level2 := add(mul(sibling2, 65537), add(mul(level1, 257), 97))
+                            }
+                            if iszero(__ite_cond) {
+                                level2 := add(mul(level1, 65537), add(mul(sibling2, 257), 97))
+                            }
+                        }
+                        let candidate := 0
+                        {
+                            let __ite_cond := sibling3OnLeft
+                            if __ite_cond {
+                                candidate := add(mul(sibling3, 65537), add(mul(level2, 257), 97))
+                            }
+                            if iszero(__ite_cond) {
+                                candidate := add(mul(level2, 65537), add(mul(sibling3, 257), 97))
+                            }
+                        }
+                        mstore(0, eq(candidate, stored))
+                        return(0, 32)
+                    }
+                    case 0x53e3f484 {
+                        /* verifyPackedPath() */
+                        if callvalue() {
+                            revert(0, 0)
+                        }
+                        if lt(calldatasize(), 196) {
+                            revert(0, 0)
+                        }
+                        if lt(calldatasize(), 196) {
+                            revert(0, 0)
+                        }
+                        let leaf := calldataload(4)
+                        let sibling0 := calldataload(36)
+                        let sibling1 := calldataload(68)
+                        let sibling2 := calldataload(100)
+                        let sibling3 := calldataload(132)
+                        let directions := calldataload(164)
+                        let stored := sload(0)
+                        let sibling0OnLeft := iszero(eq(and(directions, 1), 0))
+                        let sibling1OnLeft := iszero(eq(and(shr(1, directions), 1), 0))
+                        let sibling2OnLeft := iszero(eq(and(shr(2, directions), 1), 0))
+                        let sibling3OnLeft := iszero(eq(and(shr(3, directions), 1), 0))
                         let level0 := 0
                         {
                             let __ite_cond := sibling0OnLeft
